feat: improve matchType inference

tests/lean/run/matchtac.lean
@@ -59,3 +59,23 @@ by match h with
    | Or.inr (Or.inr h) =>
      apply Or.inl;
      assumption
+
+inductive ListLast.{u} {α : Type u} : List α → Type u
+| empty    : ListLast []
+| nonEmpty : (as : List α) → (a : α) → ListLast (as ++ [a])
+
+axiom last {α} (xs : List α) : ListLast xs
+axiom back {α} [Inhabited α] (xs : List α) : α
+axiom popBack {α} : List α → List α
+axiom backEq {α} [Inhabited α] : (xs : List α) → (x : α) → back (xs ++ [x]) = x
+axiom popBackEq {α} : (xs : List α) → (x : α) → popBack (xs ++ [x]) = xs
+
+theorem tst8 {α} [Inhabited α] (xs : List α) : xs ≠ [] → xs = popBack xs ++ [back xs] :=
+match xs, last xs with
+| _, ListLast.empty         => fun h => absurd rfl h
+| _, ListLast.nonEmpty ys y => fun _ => sorry
+
+theorem tst9 {α} [Inhabited α] (xs : List α) : xs ≠ [] → xs = popBack xs ++ [back xs] := by
+match xs, last xs with
+| _, ListLast.empty         => intro h; exact absurd rfl h
+| _, ListLast.nonEmpty ys y => intro; exact  sorry
