src/Lean/Elab/Match.lean
@@ -48,22 +48,7 @@ private def expandSimpleMatchWithType (stx discr lhsVar type rhs : Syntax) (expe
 newStx ← `(let $lhsVar : $type := $discr; $rhs);
 withMacroExpansion stx newStx $ elabTerm newStx expectedType?
 
-private def expandMatchOptTypeAux (ref : Syntax) : Nat → MacroM Syntax
-| 0   => pure $ mkHole ref
-| n+1 => do t ← expandMatchOptTypeAux n; r ← `(forall _, $t); pure (r.copyInfo ref)
-
-private def expandMatchOptType (ref : Syntax) (optType : Syntax) (numDiscrs : Nat) : MacroM Syntax :=
-if optType.isNone then
-  expandMatchOptTypeAux ref numDiscrs
-else
-  pure $ (optType.getArg 0).getArg 1
-
-private def elabMatchOptType (matchOptType : Syntax) (numDiscrs : Nat) : TermElabM Expr := do
-ref ← getRef;
-typeStx ← liftMacroM $ expandMatchOptType ref matchOptType numDiscrs;
-elabType typeStx
-
-private partial def elabDiscrsAux (discrStxs : Array Syntax) (expectedType : Expr) : Nat → Expr → Array Expr → TermElabM (Array Expr)
+private partial def elabDiscrsWitMatchTypeAux (discrStxs : Array Syntax) (expectedType : Expr) : Nat → Expr → Array Expr → TermElabM (Array Expr)
 | i, matchType, discrs =>
   if h : i < discrStxs.size then do
     let discrStx := discrStxs.get ⟨i, h⟩;
@@ -72,15 +57,40 @@ private partial def elabDiscrsAux (discrStxs : Array Syntax) (expectedType : Exp
     | Expr.forallE _ d b _ => do
       discr ← fullApproxDefEq $ elabTermEnsuringType discrStx d;
       trace `Elab.match fun _ => "discr #" ++ toString i ++ " " ++ discr ++ " : " ++ d;
-      elabDiscrsAux (i+1) (b.instantiate1 discr) (discrs.push discr)
+      elabDiscrsWitMatchTypeAux (i+1) (b.instantiate1 discr) (discrs.push discr)
     | _ => throwError ("invalid type provided to match-expression, function type with arity #" ++ toString discrStxs ++ " expected")
   else do
     unlessM (fullApproxDefEq $ isDefEq matchType expectedType) $
       throwError ("invalid result type provided to match-expression" ++ indentExpr matchType ++ Format.line ++ "expected type" ++ indentExpr expectedType);
     pure discrs
 
-private def elabDiscrs (discrStxs : Array Syntax) (matchType : Expr) (expectedType : Expr) : TermElabM (Array Expr) :=
-elabDiscrsAux discrStxs expectedType 0 matchType #[]
+private def elabDiscrsWitMatchType (discrStxs : Array Syntax) (matchType : Expr) (expectedType : Expr) : TermElabM (Array Expr) :=
+elabDiscrsWitMatchTypeAux discrStxs expectedType 0 matchType #[]
+
+private def mkUserNameFor (e : Expr) : TermElabM Name :=
+match e with
+| Expr.fvar fvarId _ => do localDecl ← getLocalDecl fvarId; pure localDecl.userName
+| _ => withFreshMacroScope do x ← `(x); pure x.getId
+
+private def elabMatchTypeAndDiscrs (discrStxs : Array Syntax) (matchOptType : Syntax) (expectedType : Expr) : TermElabM (Array Expr × Expr) :=
+let numDiscrs := discrStxs.size;
+if matchOptType.isNone then do
+  discrs ← discrStxs.mapM fun discrStx => elabTerm discrStx none;
+  matchType ← discrs.foldrM
+    (fun (discr : Expr) (matchType : Expr) => do
+      discr ← instantiateMVars discr;
+      discrType ← inferType discr;
+      discrType ← instantiateMVars discrType;
+      matchTypeBody ← kabstract matchType discr;
+      userName ← mkUserNameFor discr;
+      pure $ Lean.mkForall userName BinderInfo.default discrType matchTypeBody)
+    expectedType;
+  pure (discrs, matchType)
+else do
+  let matchTypeStx := (matchOptType.getArg 0).getArg 1;
+  matchType ← elabType matchTypeStx;
+  discrs ← elabDiscrsWitMatchType discrStxs matchType expectedType;
+  pure (discrs, matchType)
 
 /-
 nodeWithAntiquot "matchAlt" `Lean.Parser.Term.matchAlt $ sepBy1 termParser ", " >> darrow >> termParser
@@ -575,6 +585,7 @@ match val? with
   /- HACK: `fvarId` is not in the scope of `mvarId`
      If this generates problems in the future, we should update the metavariable declarations. -/
   assignExprMVar mvarId (mkFVar fvarId);
+  -- TODO: use macro scopes for creating userName
   let userName := (`_x).appendIndexAfter (s.localDecls.size+1);
   let newDecl := LocalDecl.cdecl (arbitrary _) fvarId userName type BinderInfo.default;
   modify $ fun s =>
@@ -688,9 +699,8 @@ unless result.unusedAltIdxs.isEmpty $
 
 private def elabMatchAux (discrStxs : Array Syntax) (altViews : Array MatchAltView) (matchOptType : Syntax) (expectedType : Expr)
     : TermElabM Expr := do
-matchType ← elabMatchOptType matchOptType discrStxs.size;
+(discrs, matchType) ← elabMatchTypeAndDiscrs discrStxs matchOptType expectedType;
 matchAlts ← expandMacrosInPatterns altViews;
-discrs ← elabDiscrs discrStxs matchType expectedType;
 trace `Elab.match fun _ => "matchType: " ++ matchType;
 alts ← matchAlts.mapM $ fun alt => elabMatchAltView alt matchType;
 let rhss := alts.map Prod.snd;
